Added formula_below lemmas, refactored axiom of emptyset, added axiom of subset

zfc.lean
@@ -29,6 +29,10 @@ inductive ZFC'_f1 : Type
 inductive ZFC'_f2 : Type
 | pair
 
+inductive ZFC'_rel : Type
+| ϵ
+| subset 
+
 def L_ZFC' : Language :=
 begin
 split,
@@ -42,16 +46,16 @@ exact if arityf = 0
                 else empty))   },
 {
 {intro arityr,
-exact if arityr = 2 then ZFC_rel else empty},
+exact if arityr = 2 then ZFC'_rel else empty},
 }
 end
 
 -- is there a way to do this with the equation compiler instead?
 
-lemma duh : L_ZFC'.relations 2 = ZFC_rel :=
+lemma duh : L_ZFC'.relations 2 = ZFC'_rel :=
 by refl
 
-@[reducible]def rel_is_rel : ZFC_rel → L_ZFC'.relations 2 :=
+@[reducible]def rel_is_rel : ZFC'_rel → L_ZFC'.relations 2 :=
 begin
 intro,
 simp[duh],
@@ -71,38 +75,104 @@ end
 -- prefix `∃'`:110 := _root_.fol.ex
 --set_option pp.notation true
 
-def b_not {L : Language} (n : ℕ) (f : preformula L 0) (hf : formula_below n f)  : formula_below n (fol.not f) := begin
-simp[fol.not],
-refine formula_below.b_imp _ _ _ _,
-assumption,
-exact formula_below.b_falsum
-end
+-- def b_not {L : Language} (n : ℕ) (f : preformula L 0) (hf : formula_below n f)  : formula_below n (fol.not f) := begin
+-- simp[fol.not],
+-- refine formula_below.b_imp _ _ _ _,
+-- assumption,
+-- exact formula_below.b_falsum
+-- end
+
+-- def b_and {L : Language} (n : ℕ) (f g : preformula L 0) (hf : formula_below n f) (hg : formula_below n g) : formula_below n (fol.and f g) :=
+-- begin
+-- simp[fol.and],
+-- refine b_not _ _ _,
+-- refine formula_below.b_imp _ _ _ _,
+-- assumption,
+-- apply b_not,
+-- assumption
+-- end
+
+-- def b_biimp {L : Language} (n : ℕ) (f g : preformula L 0) (hf : formula_below n f) (hg : formula_below n g) : formula_below n (f ⟺ g) :=
+-- begin
+-- simp[biimp,fol.and, fol.not],
+-- refine formula_below.b_imp _ _ _ _,
+-- have := formula_below.b_falsum, -- can we add this to _every_ local context?
+-- refine formula_below.b_imp _ _ _ _,
+-- refine formula_below.b_imp _ _ _ _,
+-- assumption, assumption,
+-- refine formula_below.b_imp _ _ _ _,
+-- refine formula_below.b_imp _ _ _ _,
+-- assumption, assumption, assumption,
+-- have := formula_below.b_falsum,
+-- assumption
+-- end
+
 
 def axiom_of_emptyset : @sentence L_ZFC' := -- for all x, x is not in the constant emptyset.
 begin
 split, swap,
   {
   dsimp[formula],
-  {exact (∀'∼(apprel (apprel (rel ZFC_rel.ϵ) &0) (func ZFC'_f0.emptyset)))},},
-  {simp*,
-have : @formula_below L_ZFC' 0 1 (fol.not (apprel (apprel (rel ZFC_rel.ϵ) &0) (func ZFC'_f0.emptyset))),
-     {
-     have : @formula_below L_ZFC' 0 1 (apprel (apprel (rel ZFC_rel.ϵ) &0) (func ZFC'_f0.emptyset)), 
-     {
-    refine formula_below.b_apprel _ _ _ _,
- swap,
-refine term_below.b_func _,
-refine formula_below.b_apprel _ _ _ _,
-refine formula_below.b_rel _,
-refine term_below.b_var _ _,
- apply nat.zero_lt_succ
-}
-,
-refine b_not _ _ _,
-exact this
-       },
-       exact (s_all (fol.not (apprel (apprel (rel $ rel_is_rel ZFC_rel.ϵ) &0) (func ZFC'_f0.emptyset))) this).snd}
+  {exact (∀'∼(apprel (apprel (rel ZFC'_rel.ϵ) &0) (func ZFC'_f0.emptyset)))},},
+
+{ simp*,
+  refine b_all _ _,
+  refine b_not _ _ _,
+  refine b_apprel _ _ _ _,
+  refine b_apprel _ _ _ _,
+  refine b_rel _,
+  refine term_below.b_var _ _,
+  simp*,
+  apply nat.zero_lt_succ,
+  refine term_below.b_func _ }
 end
+
+def axiom_of_subset : @sentence L_ZFC' := -- for all x, for all z, x ⊆ y (if and only if) , z ∈ x → z ∈ y.
+begin
+split,
+swap,
+  {
+  dsimp[formula],
+  {exact ∀' (∀'( ∀'( (apprel (apprel (rel $ rel_is_rel ZFC'_rel.subset) &0) (var 2)) ⟺ (apprel (apprel (rel ZFC'_rel.ϵ) &1) (var 2)))))}},
+{
+simp*,
+refine b_all _ _,
+refine b_all _ _,
+refine b_all _ _,
+refine b_biimp _ _ _ _ _,
+refine b_apprel _ _ _ _,
+refine b_apprel _ _ _ _,
+{refine b_rel _},
+{simp*, refine term_below.b_var _ _, apply nat.zero_lt_succ},
+{simp*, refine term_below.b_var _ _, simp*, apply nat.zero_lt_succ},
+{refine b_apprel _ _ _ _, 
+{refine b_apprel _ _ _ _,
+refine b_rel _,
+{simp*, refine term_below.b_var _ _, simp*, apply nat.zero_lt_succ}
+},
+{{simp*, refine term_below.b_var _ _, simp*, apply nat.zero_lt_succ}}
+}}
+end
+
+/- less efficient proof below -/
+--   {simp*,
+-- have : @formula_below L_ZFC' 0 1 (fol.not (apprel (apprel (rel ZFC_rel.ϵ) &0) (func ZFC'_f0.emptyset))),
+--      {
+--      have : @formula_below L_ZFC' 0 1 (apprel (apprel (rel ZFC_rel.ϵ) &0) (func ZFC'_f0.emptyset)), 
+--      {
+--     refine formula_below.b_apprel _ _ _ _,
+--  swap,
+-- refine term_below.b_func _,
+-- refine formula_below.b_apprel _ _ _ _,
+-- refine formula_below.b_rel _,
+-- refine term_below.b_var _ _,
+--  apply nat.zero_lt_succ
+-- }
+-- ,
+-- refine b_not _ _ _,
+-- exact this
+--        },
+--        exact (s_all (fol.not (apprel (apprel (rel $ rel_is_rel ZFC_rel.ϵ) &0) (func ZFC'_f0.emptyset))) this).snd}
 
 
 def axiom_of_extensionality : @sentence L_ZFC' := -- for all x for all y for all z, z in x iff z in y implies x = y
@@ -114,6 +184,8 @@ simp[formula],
 {exact sorry}
 }
 end
+
+
 
 -- etc
 
